### 1

Prove that the integral
$$
\Gamma(p) = \int_0^\infty x^{p-1} e^{-x} dx
$$
is convergent for any $p > 0$.

**Proof:**

The integral is improper at both $x=0$ and $x=\infty$. We analyze convergence at both ends.

#### Near $x=0$:
For small $x$, $e^{-x} \approx 1$, so the integrand behaves like $x^{p-1}$.

Consider:
$$
\int_0^a x^{p-1} dx = \left[ \frac{x^p}{p} \right]_0^a = \frac{a^p}{p}
$$
This is finite for any $p > 0$.

#### As $x \to \infty$:
For large $x$, $e^{-x}$ decays much faster than any power of $x$ grows. For any $p$, $x^{p-1} e^{-x} \to 0$ rapidly as $x \to \infty$.

Consider:
$$
\int_A^\infty x^{p-1} e^{-x} dx
$$
For large $x$, $e^{-x}$ dominates, so the integral converges for all $p$.

#### Conclusion:
Both at $x=0$ and $x=\infty$, the integral converges for any $p > 0$.

---


### 2

$$\dfrac{\Gamma(2/3)}{\Gamma(5/3)}$$

Apply the recursion relation twice:

$\Gamma(5/3) = (2/3)\Gamma(2/3)$

So:
$$
\frac{\Gamma(2/3)}{\Gamma(5/3)} = \frac{\Gamma(2/3)}{(2/3)\Gamma(2/3)} = \frac{3}{2}
$$

---

### 3

$$\dfrac{\Gamma(2/3)}{\Gamma(8/3)}$$

$\Gamma(8/3) = (5/3)\Gamma(5/3)$ and $\Gamma(5/3) = (2/3)\Gamma(2/3)$

So:
$$
\Gamma(8/3) = (5/3)(2/3)\Gamma(2/3) = \frac{10}{9}\Gamma(2/3)
$$
Thus:
$$
\frac{\Gamma(2/3)}{\Gamma(8/3)} = \frac{\Gamma(2/3)}{\frac{10}{9}\Gamma(2/3)} = \frac{9}{10}
$$

---

### 4

$$\dfrac{\Gamma(2/5)}{\Gamma(12/5)}$$

$\Gamma(12/5) = (7/5)\Gamma(7/5)$
$\Gamma(7/5) = (2/5)\Gamma(2/5)$

So:
$$
\Gamma(12/5) = (7/5)(2/5)\Gamma(2/5) = \frac{14}{25}\Gamma(2/5)
$$
Thus:
$$
\frac{\Gamma(2/5)}{\Gamma(12/5)} = \frac{\Gamma(2/5)}{\frac{14}{25}\Gamma(2/5)} = \frac{25}{14}
$$

---

### 5

$$\dfrac{\Gamma(1/2)\Gamma(4)}{\Gamma(9/2)}$$

$\Gamma(9/2) = (7/2)\Gamma(7/2)$
$\Gamma(7/2) = (5/2)\Gamma(5/2)$
$\Gamma(5/2) = (3/2)\Gamma(3/2)$
$\Gamma(3/2) = (1/2)\Gamma(1/2)$

$\Gamma(4) = 3! = 6$

So:
$$
\Gamma(9/2) = (7/2)(5/2)(3/2)(1/2)\Gamma(1/2) = \frac{105}{16}\Gamma(1/2)
$$
Thus:
$$
\frac{\Gamma(1/2)\Gamma(4)}{\Gamma(9/2)} = \frac{\Gamma(1/2)\cdot 6}{\frac{105}{16}\Gamma(1/2)} = \frac{6}{105/16} = \frac{96}{105} = \frac{32}{35}
$$

---

### 6

$$\dfrac{\Gamma(10)}{\Gamma(8)}$$

$\Gamma(10) = 9\Gamma(9) = 9\cdot8\Gamma(8) = 72\Gamma(8)$

So:
$$
\frac{\Gamma(10)}{\Gamma(8)} = 72
$$

---

### 7

$$
\frac{\Gamma(4)\Gamma(3/4)}{\Gamma(7/4)}
$$

**Solution:**

First, use the recursion relation:
$$
\Gamma(p+1) = p\Gamma(p)
$$

Notice that:
$$
\Gamma(7/4) = (3/4)\Gamma(3/4)
$$

Also, $\Gamma(4) = 3! = 6$.

So:
$$
\frac{\Gamma(4)\Gamma(3/4)}{\Gamma(7/4)} = \frac{6\Gamma(3/4)}{(3/4)\Gamma(3/4)} = \frac{6}{3/4} = 8
$$

---

### 8

$$\int_0^\infty x^{2/3} e^{-x} dx$$

This is already in the form of the Gamma function with $s = 2/3 + 1 = 5/3$:

- $\int_0^\infty x^{2/3} e^{-x} dx = \Gamma(5/3)$
- Numerically: $\Gamma(5/3) \approx 0.8929795$

---

### 9

$$\int_0^\infty e^{-x^4} dx$$

Let $x^4 = u \Rightarrow x = u^{1/4}, dx = \frac{1}{4} u^{-3/4} du$:

$$
\int_0^\infty e^{-x^4} dx = \int_0^\infty e^{-u} \frac{1}{4} u^{-3/4} du = \frac{1}{4} \Gamma(1/4)
$$
- Numerically: $\Gamma(1/4) \approx 3.6256099$
- So, value $\approx 0.9064025$

---

### 10

$$\int_0^\infty x^{-2/5} e^{-x} dx$$

This is $x^{s-1}$ with $s-1 = -2/5 \Rightarrow s = 3/5$:

- $\int_0^\infty x^{-2/5} e^{-x} dx = \Gamma(3/5)$
- Numerically: $\Gamma(3/5) \approx 1.4891922$

---

### 11

$$\int_0^\infty x^5 e^{-x^2} dx$$

Let $x^2 = u \Rightarrow x = u^{1/2}, dx = \frac{1}{2} u^{-1/2} du$:

$$
\int_0^\infty x^5 e^{-x^2} dx = \int_0^\infty u^{5/2} e^{-u} \frac{1}{2} u^{-1/2} du = \frac{1}{2} \int_0^\infty u^2 e^{-u} du = \frac{1}{2} \Gamma(3)
$$
- $\Gamma(3) = 2! = 2$
- So, value = 1

---

### 12

$$\int_0^\infty x e^{-x^3} dx$$

Let $x^3 = u \Rightarrow x = u^{1/3}, dx = \frac{1}{3} u^{-2/3} du$:

$$
\int_0^\infty x e^{-x^3} dx = \int_0^\infty u^{1/3} e^{-u} \frac{1}{3} u^{-2/3} du = \frac{1}{3} \int_0^\infty u^{-1/3} e^{-u} du = \frac{1}{3} \Gamma(2/3)
$$
- Numerically: $\Gamma(2/3) \approx 1.3541179$
- So, value $\approx 0.4513726$

---

### 13

$$\int_0^1 x^2 \left( \ln \frac{1}{x} \right)^3 dx$$

Let $x = e^{-u} \Rightarrow dx = -e^{-u} du, x^2 = e^{-2u}, \ln(1/x) = u$:

Limits: $x=0 \to u=\infty, x=1 \to u=0$

$$
\int_0^1 x^2 (\ln(1/x))^3 dx = \int_{\infty}^0 e^{-2u} u^3 (-e^{-u}) du = \int_0^{\infty} u^3 e^{-3u} du
$$
Let $t = 3u \Rightarrow du = dt/3$:

$$
= \int_0^{\infty} \left(\frac{t}{3}\right)^3 e^{-t} \frac{dt}{3} = \frac{1}{81} \int_0^{\infty} t^3 e^{-t} dt = \frac{1}{81} \Gamma(4)
$$
- $\Gamma(4) = 3! = 6$
- So, value = $6/81 = 2/27 \approx 0.074074$

---

### 14

$$\int_0^1 \sqrt[3]{\ln x} dx$$

Let $t = -\ln x \Rightarrow x = e^{-t}, dx = -e^{-t} dt$

Limits: $x=0 \to t=\infty, x=1 \to t=0$

$$
\int_0^1 (\ln x)^{1/3} dx = \int_{\infty}^0 (-t)^{1/3} (-e^{-t}) dt = \int_0^{\infty} t^{1/3} e^{-t} dt = \Gamma(4/3)
$$
- Numerically: $\Gamma(4/3) \approx 0.8929795$

---

### 15

$$\int_0^\infty x^{-1/3} e^{-8x} dx$$

This is $x^{s-1} e^{-\lambda x}$ with $s-1 = -1/3 \Rightarrow s = 2/3$, $\lambda = 8$:

$$
\int_0^\infty x^{-1/3} e^{-8x} dx = 8^{-2/3} \Gamma(2/3)
$$
- $8^{-2/3} = (2^3)^{-2/3} = 2^{-2} = 1/4$
- $\Gamma(2/3) \approx 1.3541179$
- So, value $\approx 0.3385295$

---

### 16

A particle starting from rest at $x = 1$ moves along the $x$ axis toward the origin. Its potential energy is $V = \frac{1}{2}m \ln x$. Write the Lagrange equation and integrate it to find the time required for the particle to reach the origin.

**Solution:**

The Lagrangian is:
$$
L = T - V = \frac{1}{2}m \dot{x}^2 - \frac{1}{2}m \ln x
$$

Since $L$ does not depend explicitly on time, use conservation of energy:
$$
E = T + V = \text{constant}
$$

At $x=1$, the particle starts from rest, so $\dot{x}_0 = 0$:
$$
E = 0 + \frac{1}{2}m \ln 1 = 0
$$

At any $x$:
$$
\frac{1}{2}m \dot{x}^2 + \frac{1}{2}m \ln x = 0
$$
$$
\dot{x}^2 = -\ln x
$$

Since $\dot{x} < 0$ (moving toward the origin):
$$
\dot{x} = -\sqrt{-\ln x}
$$

So:
$$
\frac{dx}{dt} = -\sqrt{-\ln x}
$$

Separate variables and integrate from $x=1$ to $x=0$ (and $t=0$ to $t_f$):
$$
\int_1^0 \frac{dx}{-\sqrt{-\ln x}} = \int_0^{t_f} dt
$$
$$
\int_0^1 \frac{dx}{\sqrt{-\ln x}} = t_f
$$

Let $u = -\ln x \implies x = e^{-u}, dx = -e^{-u} du$

When $x=1$, $u=0$; when $x=0$, $u=\infty$:
$$
\int_{x=0}^{x=1} \frac{dx}{\sqrt{-\ln x}} = \int_{u=\infty}^{u=0} \frac{-e^{-u} du}{\sqrt{u}}
$$
$$
= \int_{u=0}^{u=\infty} \frac{e^{-u}}{\sqrt{u}} du = \int_0^{\infty} u^{-1/2} e^{-u} du = \Gamma\left(\frac{1}{2}\right)
$$

**Final answer:**
$$
t_f = \Gamma\left(\frac{1}{2}\right)
$$

Where $\Gamma(1/2) = \sqrt{\pi} \approx 1.77245$.

---

### 17

Express as a Gamma function:
$$
\int_0^1 \left[ \ln \left( \frac{1}{x} \right) \right]^{p-1} dx
$$

**Solution:**

Let $u = \ln\left(\frac{1}{x}\right) = -\ln x$, so $x = e^{-u}$ and $dx = -e^{-u} du$.

When $x=0$, $u=\infty$; when $x=1$, $u=0$.

So:
$$
\int_0^1 [\ln(1/x)]^{p-1} dx = \int_{u=\infty}^{u=0} u^{p-1} (-e^{-u}) du = \int_0^{\infty} u^{p-1} e^{-u} du = \Gamma(p)
$$

**Final answer:**
$$
\int_0^1 \left[ \ln \left( \frac{1}{x} \right) \right]^{p-1} dx = \Gamma(p)
$$

---

